@prefix foaf:      <http://xmlns.com/foaf/0.1/> .
@prefix rdfs:      <http://www.w3.org/2000/01/rdf-schema#> .
@prefix owl:       <http://www.w3.org/2002/07/owl#> .
@prefix rdf:       <http://www.w3.org/1999/02/22-rdf-syntax-ns#> .
@prefix italy:     <http://data.kasabi.com/dataset/italy/> .
@prefix eurostat:  <http://ec.europa.eu/eurostat/ramon/ontologies/geographic.rdf#> .

#
# Vocabulary: Region, Province, Comune
#

italy:Region
    rdf:type rdfs:Class ;
    rdf:type owl:Class ;
    rdfs:subClassOf <http://dbpedia.org/resource/Category:Types_of_country_subdivisions> ;
    rdfs:label "Region"@en ;
    rdfs:label "Regione"@it ;
    rdfs:comment "A geographical region (i.e. the first-level administrative divisions of a state). For example, Italy is divided in 20 regions."@en ;
    rdfs:comment "Una regione costituisce il primo livello di suddivisione di uno stato. L'Italia, per esempio, e' suddivisa in 20 regioni."@it ;
    owl:sameAs <http://dbpedia.org/resource/Region_of_Italy> ;
    owl:sameAs <http://rdf.freebase.com/ns/m/0fg5q> ;
    owl:sameAs <http://dbpedia.org/resource/Italian_NUTS_level_1_regions> ;
    owl:sameAs <http://dbpedia.org/class/yago/RegionsOfItaly> ;
    foaf:page <http://en.wikipedia.org/wiki/Region_of_Italy> ;
    rdfs:seeAlso <http://en.wikipedia.org/wiki/index.html?curid=55633> ;
    rdfs:seeAlso <http://en.wikipedia.org/wiki/Region> ;
    rdfs:seeAlso <http://en.wikipedia.org/wiki/Region_of_Italy> ;
    .

italy:Province
    rdf:type rdfs:Class ;
    rdf:type owl:Class ;
    rdfs:subClassOf <http://dbpedia.org/resource/Category:Types_of_country_subdivisions> ;
    rdfs:label "Province"@en ;
    rdfs:label "Provincia"@it ;
    rdfs:comment "In Italy is an administrative division of intermediate level between a municipality (comune) and a region (regione)."@en ;
    rdfs:comment "Ente locale territoriale il cui territorio è per estensione inferiore a quello della regione (della quale, a sua volta, fa parte) e comprende il territorio di più comuni."@it ;
    owl:sameAs <http://dbpedia.org/resource/Provinces_of_Italy> ;
    owl:sameAs <http://rdf.freebase.com/ns/m/0fkxj> ;
    owl:sameAs <http://dbpedia.org/class/yago/ProvincesOfItaly> ;
    foaf:page <http://en.wikipedia.org/wiki/Provinces_of_Italy> ;
    rdfs:seeAlso <http://en.wikipedia.org/wiki/index.html?curid=15489197> ;
    rdfs:seeAlso <http://en.wikipedia.org/wiki/Province> ;
    rdfs:seeAlso <http://en.wikipedia.org/wiki/Provinces_of_Italy> ;
    .

italy:Comune
    rdf:type rdfs:Class ;
    rdf:type owl:Class ;
    rdfs:subClassOf <http://dbpedia.org/resource/Category:Types_of_country_subdivisions> ;
    rdfs:label "Municipality"@en ;
    rdfs:label "Comune"@it ;
    rdfs:comment "In Italy, the 'comune' is the basic administrative division, and may be approximated in casual speech by the English word township or municipality."@en ;
    rdfs:comment "In Italia il comune è un ente locale autonomo ed indipendente. Può essere suddiviso in frazioni ed appartiene a una provincia."@it ;
    owl:sameAs <http://dbpedia.org/resource/Comune> ;
    owl:sameAs <http://rdf.freebase.com/ns/m/02bsc3> ;
    owl:sameAs <http://dbpedia.org/class/yago/MunicipalitiesOfItaly> ;
    foaf:page <http://en.wikipedia.org/wiki/Comune> ;
    rdfs:seeAlso <http://en.wikipedia.org/wiki/index.html?curid=457055> ;
    rdfs:seeAlso <http://en.wikipedia.org/wiki/Comune> ;
    rdfs:seeAlso <http://en.wikipedia.org/wiki/List_of_comuni_of_Italy> ;
    .

#
# Small additions 
#

italy:aosta eurostat:regionCode "ITF20" .
italy:lazio rdfs:label "Lazio"@en .
italy:molise rdfs:label "Molise"@en .
italy:emilia-romagna rdfs:label "Emilia-Romagna"@en .

#
# Links
#

italy:sicilia
    owl:sameAs <http://dbpedia.org/resource/Sicilia> ;
    owl:sameAs <http://sws.geonames.org/2523119/> ;
    owl:sameAs <http://sw.opencyc.org/concept/Mx4rvVifXpwpEbGdrcN5Y29ycA> ;
    owl:sameAs <http://rdf.freebase.com/ns/m/06w92> ;
    owl:sameAs <http://rdf.freebase.com/ns/en.sicily> ;
    owl:sameAs <http://rdf.freebase.com/ns/guid.9202a8c04000641f8000000000036d22> ;
    owl:sameAs <http://www4.wiwiss.fu-berlin.de/eurostat/page/regions/Sicilia> ;
    owl:sameAs <http://ec.europa.eu/eurostat/ramon/rdfdata/nuts2008/ITG1> ;
    owl:sameAs <http://data.nytimes.com/66897629118838755101> ;
    owl:sameAs <http://yago-knowledge.org/resource/Sicily> ;
    foaf:page <http://en.wikipedia.org/wiki/Sicily> ;
    foaf:isPrimaryTopicOf <http://kasabi.com/dataset/italy/sicilia.html> ; ## ???
    rdfs:seeAlso <urn:/wikipedia/en_title:Sicily> ;
    rdfs:seeAlso <urn:/wikipedia/it_title:Sicilia> ;
    rdfs:seeAlso <http://www.w3.org/2006/03/wn/wn20/instances/wordsense-Sicily-noun-2.rdf> ;
    .
